[{a}]

$$<<< \int \dfrac{1}{1-\sin^2 x}\dd x$$

+++
Solución
+++

$$<<< 
\int \dfrac{1}{1-\sin^2 x}\dd x \\
\qquad = \int \dfrac{1}{\cos^2 x}\dd x \\
\qquad = \hl{\tan x+k}
$$

+++

---
[{b}]

$$<<< \int \dfrac{7x^4-3x^2-3x+5}{4x^2}\dd x$$

+++
Solución
+++

$$<<< 
\int \dfrac{7x^4-3x^2-3x+5}{4x^2}\dd x \\
\qquad = \int \left(\dfrac{7}{4}x^2-\dfrac{3}{4}-\dfrac{3}{4}\dfrac{1}{x}+\dfrac{5}{4}\dfrac{1}{x^2}\right)\dd x \\
\qquad = \hl{\dfrac{7}{12}x^3-\dfrac{3}{4}x-\dfrac{3}{4}\ln|x|-\dfrac{5}{4x}+k}
$$

+++

---
[{c}]

$$<<< \int \dfrac{1+7x^2-5x^3}{2\sqrt{x}}\dd x$$

+++
Solución
+++

$$<<< 
\int \dfrac{1+7x^2-5x^3}{2\sqrt{x}}\dd x \\
\qquad = \int \left(\dfrac{1}{2}x^{-\frac{1}{2}}+\dfrac{7}{2}x^{\frac{3}{2}}-\dfrac{5}{2}x^{\frac{5}{2}}\right)\dd x \\
\qquad = \dfrac{1}{2}\left(\dfrac{1}{2}\right)^{-1}x^{\frac{1}{2}}+\dfrac{7}{2}\left(\dfrac{5}{2}\right)^{-1}x^{\frac{5}{2}}-\dfrac{5}{2}\left(\dfrac{7}{2}\right)^{-1}x^{\frac{7}{2}}+k \\
\qquad = \hl{x^{\frac{1}{2}}+\dfrac{7}{5}x^{\frac{5}{2}}-\dfrac{5}{7}x^{\frac{7}{2}}+k}
$$

+++

---
[{d}]

$$<<< \int \dfrac{3x+4\sqrt[4]{x}}{5\sqrt[3]{x}}\dd x$$

+++
Solución
+++

$$<<< 
\int \dfrac{3x+4\sqrt[4]{x}}{5\sqrt[3]{x}}\dd x \\
\qquad = \int \dfrac{3x+4x^{\frac{1}{4}}}{5x^{\frac{1}{3}}}\dd x \\
\qquad = \int \left(\dfrac{3}{5}x^{\frac{2}{3}}+\dfrac{4}{5}x^{-\frac{1}{12}}\right)\dd x \\
\qquad = \dfrac{3}{5}\left(\dfrac{5}{3}\right)^{-1}x^{\frac{5}{3}}+\dfrac{4}{5}\left(\dfrac{11}{12}\right)^{-1}x^{\frac{11}{12}}+k \\
\qquad = \hl{\dfrac{9}{25}x^{\frac{5}{3}}+\dfrac{48}{55}x^{\frac{11}{12}}+k}
$$

+++

---
[{e}]

$$<<< \int \dfrac{4\sqrt{x}-3\sqrt[5]{x^3}}{3\sqrt[3]{x^2}}\dd x$$

+++
Solución
+++

$$<<< 
\int \dfrac{4\sqrt{x}-3\sqrt[5]{x^3}}{3\sqrt[3]{x^2}}\dd x \\
\qquad = \int \dfrac{4x^{\frac{1}{2}}-3x^{\frac{3}{5}}}{3x^{\frac{2}{3}}}\dd x \\
\qquad = \int \left(\dfrac{4}{3}x^{-\frac{1}{6}}-x^{-\frac{1}{15}}\right)\dd x \\
\qquad = \dfrac{4}{3}\left(\dfrac{5}{6}\right)^{-1}x^{\frac{5}{6}}-\left(\dfrac{14}{15}\right)^{-1}x^{\frac{14}{15}}+k \\
\qquad = \hl{\dfrac{8}{5}x^{\frac{5}{6}}-\dfrac{15}{14}x^{\frac{14}{15}}+k}
$$

+++