[{a}]

$$<<< \left[\ln\left(\dfrac{1+x}{1-x}\right)\right]' $$

+++
Solution
+++

$$<<< 
\left[\ln\left(\dfrac{1+x}{1-x}\right)\right]'
\\ \qquad 
= \dfrac{1-x}{1+x}\left[\dfrac{1+x}{1-x}\right]'
\\ \qquad 
= \dfrac{1-x}{1+x}\dfrac{[1+x]'(1-x)-(1+x)[1-x]'}{(1-x)^2}
\\ \qquad 
= \dfrac{1-x}{1+x}\dfrac{(1-x)+(1+x)}{(1-x)^2}
\\ \qquad 
= \hl{\dfrac{2}{(1+x)(1-x)}}
$$

Alternatively,

$$<<< 
\left[\ln\left(\dfrac{1+x}{1-x}\right)\right]'
\\ \qquad 
= [\ln(1+x)-\ln(1+x)]'
\\ \qquad 
= \dfrac{1}{1+x}[1+x]'-\dfrac{1}{1-x}[1-x]'
\\ \qquad 
= \dfrac{1}{1+x}+\dfrac{1}{1-x}
\\ \qquad 
= \dfrac{(1-x)+(1+x)}{(1+x)(1-x)}
\\ \qquad 
= \hl{\dfrac{2}{(1+x)(1-x)}}
$$

+++

---
[{b}]

$$<<< \left[\dfrac{x\sin(2x)}{\tan(3x)}\right]' $$

+++
Solution
+++

$$<<< 
\left[\dfrac{x\sin(2x)}{\tan(3x)}\right]'
\\ \qquad 
= \dfrac{[x\sin(2x)]'(\tan(3x))-(x\sin(2x))[\tan(3x)]'}{(\tan(3x))^2}
\\ \qquad 
= \dfrac{(\sin(2x)+2x\cos(2x))(\tan(3x))-(x\sin(2x))\left(\frac{3}{\cos^2(3x)}\right)}{\tan^2(3x)}
\\ \qquad 
= \hl{\dfrac{\sin(2x)+2x\cos(2x)}{\tan(3x)}-\dfrac{3x\sin(2x)}{\sin^2(3x)}}
$$

+++

---
[{c}]

$$<<< \left[\sin\left(\dfrac{x}{x+\sin x}\right)\right]'$$

+++
Solution
+++

$$<<< 
\left[\sin\left(\dfrac{x}{x+\sin x}\right)\right]'
\\ \qquad 
= \cos\left(\dfrac{x}{x+\sin x}\right)\left[\dfrac{x}{x+\sin x}\right]'
\\ \qquad 
= \cos\left(\dfrac{x}{x+\sin x}\right)\dfrac{[x]'(x+\sin x)-x[x+\sin x]'}{(x+\sin x)^2}
\\ \qquad 
= \cos\left(\dfrac{x}{x+\sin x}\right)\dfrac{(x+\sin x)-x(1+\cos x)}{(x+\sin x)^2}
\\ \qquad 
= \hl{\cos\left(\dfrac{x}{x+\sin x}\right)\dfrac{\sin x-x\cos x}{(x+\sin x)^2}}
$$

+++

---
[{d}]

$$<<< \left[\cos^3(1-x^2)\right]' $$

+++
Solution
+++

$$<<< 
\left[\cos^3(1-x^2)\right]'
\\ \qquad 
= 3\cos^2(1-x^2)[\cos(1-x^2)]'
\\ \qquad 
= -3\cos^2(1-x^2)\sin(1-x^2)[1-x^2]
\\ \qquad 
= \hl{6x\cos^2(1-x^2)\sin(1-x^2)}
$$

+++

---
[{e}]

$$<<< \left[\sqrt[3]{x+\sqrt{3x}}\right]' $$

+++
Solution
+++

$$<<< 
\left[\sqrt[3]{x+\sqrt{3x}}\right]'
\\ \qquad 
= (x+\sqrt{3x})^{\frac{1}{3}}
\\ \qquad 
= \dfrac{1}{3}(x+\sqrt{3x})^{-\frac{2}{3}}[x+\sqrt{3x}]'
\\ \qquad 
= \hl{\dfrac{1}{3}(x+\sqrt{3x})^{-\frac{2}{3}}\left(1+\dfrac{\sqrt{3}}{2\sqrt{x}}\right)}
$$

+++