[{a}]

$$<<< [(x^3-x)\sin x]' $$

+++
Solution
+++

$$<<< 
[(x^3-x)\sin x]'
\\ \qquad 
= [x^3-x]'\sin x + (x^3-x)[\sin x]'
\\ \qquad 
= \hl{(3x^2-1)\sin x + (x^3-x)\cos x}
$$

+++

---
[{b}]

$$<<< [\sin x\ln x]' $$

+++
Solution
+++

$$<<< 
[\sin x\ln x]'
\\ \qquad 
= [\sin x]'\ln x + \sin x[\ln x]'
\\ \qquad 
= \hl{\cos x\ln x + \dfrac{\sin x}{x}}
$$

+++

---
[{c}]

$$<<< [x^2 2^x]' $$

+++
Solution
+++

$$<<< 
[x^2 2^x]'
\\ \qquad 
= [x^2]'2^x + x^2[2^x]'
\\ \qquad 
= 2x\cdot 2^x + x^2 2^x\ln(2)
\\ \qquad 
= \hl{(2x+\ln(2)x^2)2^x}
$$

+++

---
[{d}]

$$<<< \left[\dfrac{3x^3-2x}{x^2+3x-1}\right]' $$

+++
Solution
+++

$$<<< 
\left[\dfrac{3x^3-2x}{x^2+3x-1}\right]'
\\ \qquad 
= \dfrac{[3x^3-2x]'(x^2+3x-1)-(3x^3-2x)[x^2+3x-1]'}{(x^2+3x-1)^2}
\\ \qquad 
= \dfrac{(9x^2-2)(x^2+3x-1)-(3x^3-2x)(2x+3)}{(x^2+3x-1)^2}
\\ \qquad 
= \dfrac{(9x^4+27x^3-9x^2-2x^2-6x+2)-(6x^4+9x^3-4x^2-6x)}{(x^2+3x-1)^2}
\\ \qquad 
= \hl{\dfrac{3x^4+18x^3-7x^2+2}{(x^2+3x-1)^2}}
$$

+++

---
[{e}]

$$<<< \left[\dfrac{5x^2-3x}{x\sin x}\right]'$$

+++
Solution
+++

$$<<< 
\left[\dfrac{5x^2-3x}{x\sin x}\right]'
\\ \qquad 
= \left[\dfrac{5x-3}{\sin x}\right]'
\\ \qquad 
= \dfrac{[5x-3]'(\sin x)-(5x-3)[\sin x]'}{(\sin x)^2}
\\ \qquad 
= \dfrac{(5)(\sin x)-(5x-3)(\cos x)}{\sin^2(x)}
\\ \qquad 
= \hl{\dfrac{5}{\sin(x)}+\dfrac{(3-5x)\cos x}{\sin^2(x)}}
$$

+++